

Script for the equations of motion of a T orsobot with rimless wheel

Constants:

L : Spoke length

l : distance of torso CoM from the wheel center

I_w : Moment of inertia of the wheel along the out of plane axis (y), about wheel CoM

I_t : Moment of inertia of the torso along the out of plane axis (y), about torso CoM

M : mass of the wheel

m : mass of the torso

State variables:

θ : angle of wheel with respect to slope normal

ϕ : angle of the torso with respect to slope normal

$\dot{\theta}$: angular rate of the wheel

$\dot{\phi}$: angular rate of the torso

State vectors

$$q = \begin{bmatrix} \theta \\ \phi \\ \dot{\theta} \\ \dot{\phi} \end{bmatrix}$$

$$\dot{q} = \begin{bmatrix} \dot{\theta} \\ \dot{\phi} \\ \ddot{\theta} \\ \ddot{\phi} \end{bmatrix} = \begin{bmatrix} q_3 \\ q_4 \\ f_3(q, u) \\ f_4(q, u) \end{bmatrix}$$

$$\dot{q} = f(q, u)$$

Stance Dynamics

During stance, equations of motion are derived using Newton-Euler equations.

$$q := \text{Vector}([q1, q2, q3, q4])$$

$$q := \begin{bmatrix} q1 \\ q2 \\ q3 \\ q4 \end{bmatrix}$$

(1)

$$R := m \cdot l \cdot L \cdot \cos(q1 - q2)$$

$$R := m \, l \, L \cos(q1 - q2) \quad (2)$$

$$S := m \cdot l^2 + I_t$$

$$S := l^2 \, m + I_t \quad (3)$$

$$V := \text{simplify}(m \cdot L^2 + M \cdot L^2 + I_w)$$

$$V := I_w + (m + M) \, L^2 \quad (4)$$

$$f1 := m \cdot l \cdot L \cdot q3^2 \cdot \sin(q1 - q2) + m \cdot g \cdot l \cdot \sin(\alpha + q2)$$

$$f1 := m \, l \, L \, q3^2 \sin(q1 - q2) + m \, g \, l \sin(\alpha + q2) \quad (5)$$

$$f2 := m \cdot l \cdot L \cdot q4^2 \cdot \sin(q2 - q1) + (m + M) \cdot g \cdot L \cdot \sin(\alpha + q1)$$

$$f2 := -m \, l \, L \, q4^2 \sin(q1 - q2) + (m + M) \, g \, L \sin(\alpha + q1) \quad (6)$$

$$N := \text{Matrix}([[1, 0, 0, 0], [0, 1, 0, 0], [0, 0, R, S], [0, 0, V, R]])$$

$$N := \begin{bmatrix} 1 & 0 & 0 & 0 \\ 0 & 1 & 0 & 0 \\ 0 & 0 & m \, l \, L \cos(q1 - q2) & l^2 \, m + I_t \\ 0 & 0 & I_w + (m + M) \, L^2 & m \, l \, L \cos(q1 - q2) \end{bmatrix} \quad (7)$$

$$f := \text{Vector}([q3, q4, f1, f2])$$

$$f := \begin{bmatrix} q3 \\ q4 \\ m \, l \, L \, q3^2 \sin(q1 - q2) + m \, g \, l \sin(\alpha + q2) \\ -m \, l \, L \, q4^2 \sin(q1 - q2) + (m + M) \, g \, L \sin(\alpha + q1) \end{bmatrix} \quad (8)$$

$$H := \text{Vector}([0, 0, -1, 1])$$

$$H := \begin{bmatrix} 0 \\ 0 \\ -1 \\ 1 \end{bmatrix} \quad (9)$$

$$q_dot := \text{LinearAlgebra}[\text{MatrixInverse}](N). (f + H \cdot T)$$

$$q_dot := \quad (10)$$

$$\begin{bmatrix} \dots \\ \dots \\ \frac{m \, l \, L \cos(q1 - q2) \left(-T + m \, l \, L \, q3^2 \sin(q1 - q2) + m \, g \, l \sin(\alpha + q1) \right)}{m^2 \, l^2 \, L^2 \cos(q1 - q2)^2 - L^2 \, M \, l^2 \, m - L^2 \, l^2 \, m^2 - I_l \, L^2 \, M - I_l \, L^2 \, m - I_l \, m^2} \dots \\ \frac{\left(-L^2 \, M - L^2 \, m - I_w \right) \left(-T + m \, l \, L \, q3^2 \sin(q1 - q2) + m \, g \, l \sin(\alpha + q1) \right)}{m^2 \, l^2 \, L^2 \cos(q1 - q2)^2 - L^2 \, M \, l^2 \, m - L^2 \, l^2 \, m^2 - I_l \, L^2 \, M - I_l \, L^2 \, m - I_l \, m^2} \dots \end{bmatrix}$$

$q_dot := simplify(q_dot)$
 $q_dot :=$ (11)

$$\begin{bmatrix} \dots \\ \dots \\ \frac{-m \, l \, L \cos(q1 - q2) \left(-T + m \, l \, L \, q3^2 \sin(q1 - q2) + m \, g \, l \sin(\alpha + q1) \right)}{-m^2 \, l^2 \, L^2 \cos(q1 - q2)^2 - L^2 \, M \, l^2 \, m - L^2 \, l^2 \, m^2 - I_l \, L^2 \, M - I_l \, L^2 \, m - I_l \, m^2} \dots \\ \frac{m \left(-T + m \, l \, L \, q4^2 \sin(q1 - q2) - (m + M) \, g \, L \sin(\alpha + q1) \right) \, L \, l \, \cos(q1 - q2)}{-m^2 \, l^2 \, L^2 \cos(q1 - q2)^2 - L^2 \, M \, l^2 \, m - L^2 \, l^2 \, m^2 - I_l \, L^2 \, M - I_l \, L^2 \, m - I_l \, m^2} \dots \end{bmatrix}$$

$A := VectorCalculus[Jacobian](q_dot, convert(q, list))$
 $A :=$ (12)

$$\begin{bmatrix} \dots \\ \dots \\ \frac{m \, l \, L \sin(q1 - q2)}{m^2 \, l^2 \, L^2 \cos(q1 - q2)^2 - L^2 \, M \, l^2 \, m - L^2 \, l^2 \, m^2 - I_l \, L^2 \, M - I_l \, L^2 \, m - I_l \, m^2} \dots \\ \frac{m \left(m \, l \, L \, q4^2 \cos(q1 - q2) - (m + M) \, g \, L \sin(\alpha + q1) \right)}{m^2 \, l^2 \, L^2 \cos(q1 - q2)^2 - L^2 \, M \, l^2 \, m - L^2 \, l^2 \, m^2 - I_l \, L^2 \, M - I_l \, L^2 \, m - I_l \, m^2} \dots \end{bmatrix}$$

$A := eval(A, [q1=0, q2=0, q3=0, q4=0, T=0])$
 $A :=$ (13)

$$\begin{bmatrix} 0 & \dots \\ 0 & \dots \\ \frac{(l^2 m + I_l) (m + M) g L \cos(\alpha)}{-L^2 l^2 m^2 + (l^2 m + I_l) (I_w + (m + M) L^2)} & - \frac{m^2 l}{-L^2 l^2 m^2 + (l^2 m + I_l) (I_w + (m + M) L^2)} \dots \\ - \frac{m (m + M) g L^2 \cos(\alpha) l}{-L^2 l^2 m^2 + (l^2 m + I_l) (I_w + (m + M) L^2)} & \frac{m g l \cos(\alpha)}{-L^2 l^2 m^2 + (l^2 m + I_l) (I_w + (m + M) L^2)} \dots \end{bmatrix}$$

Stance Dynamics

During collision, momentum is preserved about the collision point.

Before collision, the velocity of the center of mass of the wheel

$$vg1 := Vector([L \cdot q3 \cdot \cos(q1), 0, -L \cdot q3 \cdot \sin(q1)])$$

$$vg1 := \begin{bmatrix} L q3 \cos(q1) \\ 0 \\ -L q3 \sin(q1) \end{bmatrix} \quad (14)$$

$$vg2 := Vector([L \cdot q3 \cdot \cos(q1) + l \cdot q4 \cdot \cos(q2), 0, -(L \cdot q3 \cdot \sin(q1) + l \cdot q4 \cdot \sin(q2))])$$

$$vg2 := \begin{bmatrix} L q3 \cos(q1) + l q4 \cos(q2) \\ 0 \\ -L q3 \sin(q1) - l q4 \sin(q2) \end{bmatrix} \quad (15)$$

$$rg1 := Vector([-L \cdot \sin(q1), 0, L \cdot \cos(q1)])$$

$$rg1 := \begin{bmatrix} -L \sin(q1) \\ 0 \\ L \cos(q1) \end{bmatrix} \quad (16)$$

$$rg2 := Vector([(-L \cdot \sin(q1) + l \cdot \sin(q2)), 0, (L \cdot \cos(q1) + l \cdot \cos(q2))])$$

$$rg2 := \begin{bmatrix} -L \sin(q1) + l \sin(q2) \\ 0 \\ L \cos(q1) + l \cos(q2) \end{bmatrix} \quad (17)$$

$$mom_1 := simplify(LinearAlgebra[CrossProduct](M \cdot rg1, vg1))$$

$$mom_1 := \begin{bmatrix} 0 \\ M q3 L^2 \cos(2 q1) \\ 0 \end{bmatrix} \quad (18)$$

$$mom_2 := (LinearAlgebra[CrossProduct](m \cdot rg2, vg2))$$

$$mom_2 := \begin{bmatrix} 0 & \dots \\ -m (-L \sin(q1) + l \sin(q2)) (-L q3 \sin(q1) - l q4 \sin(q2)) + m (L \cos(q1) \dots \\ 0 & \dots \end{bmatrix} \quad (19)$$

$$RHS := (Vector([0, I_t \cdot q4, 0]) + Vector([0, I_w \cdot q3, 0]) + mom_1 + mom_2)$$

$$RHS := \begin{bmatrix} \dots \\ I_t q4 + I_w q3 + M q3 L^2 \cos(2 q1) - m (-L \sin(q1) + l \sin(q2)) (-L \dots \\ \dots \end{bmatrix} \quad (20)$$

The vector \mathbf{q} denotes the state right before collision (it could also be represented by \mathbf{q}^-)

The vector \mathbf{q}^+ represents the state right after collision

$$\mathbf{R}(\mathbf{q}) \cdot \mathbf{q}^+ = s(\mathbf{q}^-)$$

$$F := (m + M) \cdot L \cdot \sin(q1)$$

$$F := (m + M) L \sin(q1) \quad (21)$$

$$G := -m \cdot l \cdot \sin(q2)$$

$$G := -m l \sin(q2) \quad (22)$$

$$s1 := -F \cdot q3 + G \cdot q4$$

$$s1 := -(m + M) L \sin(q1) q3 - m l \sin(q2) q4 \quad (23)$$

$$Q := I_w + M \cdot L^2 + m \cdot L^2 + m \cdot l \cdot L \cdot (\cos(q1 + q2))$$

$$Q := I_w + L^2 M + L^2 m + m l L \cos(q1 + q2) \quad (24)$$

$$P := I_t + m \cdot l^2 + m \cdot l \cdot L \cdot (\cos(q1 + q2))$$

$$P := I_t + l^2 m + m l L \cos(q1 + q2) \quad (25)$$

$$s2 := (I_w + L^2 \cdot (m + M) \cdot \cos(2 \cdot q1) + m \cdot l \cdot L \cdot (\cos(q1 - q2))) \cdot q3 + P \cdot q4$$

$$s2 := (I_w + L^2 (m + M) \cos(2 q1) + m l L \cos(q1 - q2)) q3 + (I_t + l^2 m + m l L \cos(q1 + q2)) q4 \quad (26)$$

$$R := Matrix([[1, 0, 0, 0], [0, 1, 0, 0], [0, 0, F, G], [0, 0, Q, P]])$$

$$R := \quad (27)$$

$$\begin{aligned}
 & \begin{bmatrix} 1 & 0 & 0 & 0 & \cdots \\ 0 & 1 & 0 & 0 & \cdots \\ 0 & 0 & (m+M)L\sin(q1) & -ml\sin(q2) & \cdots \\ 0 & 0 & I_w + L^2 M + L^2 m + mlL\cos(q1+q2) & I_t + I^2 m + mlL\cos(q1+q2) & \cdots \end{bmatrix} \\
 & s := \text{Vector}([-q1, q2, s1, s2]) \\
 & s := \hspace{15em} \textbf{(28)}
 \end{aligned}$$

$$\begin{aligned}
 & \begin{bmatrix} -q1 & \cdots \\ q2 & \cdots \\ -(m+M)L\sin(q1)q3 - ml\sin(q2)q4 & \cdots \\ (I_w + L^2(m+M)\cos(2q1) + mlL\cos(q1-q2))q3 + (I_t + I^2 m + mlL\cos(q1+q2))q4 & \cdots \end{bmatrix} \\
 & q_after := \text{LinearAlgebra}[\text{MatrixInverse}](R). (s) \\
 & q_after := \hspace{15em} \textbf{(29)}
 \end{aligned}$$

$$\begin{aligned}
 & \begin{bmatrix} \cdots \\ \cdots \\ \frac{L^2 M \sin(q1) \cos(q1+q2) l m + L^2 m^2 \cos^2(q1+q2)}{L^2 M \sin(q1) \cos(q1+q2) l m + L^2 m^2 \cos^2(q1+q2)} \cdots \\ \frac{L^2 M \sin(q1) \cos(q1+q2) l m + L^2 m^2 \cos^2(q1+q2)}{L^2 M \sin(q1) \cos(q1+q2) l m + L^2 m^2 \cos^2(q1+q2)} \cdots \end{bmatrix} \\
 & q_after := \text{simplify}(q_after) \\
 & q_after := \hspace{15em} \textbf{(30)}
 \end{aligned}$$

$$\left[\begin{array}{c} \dots \\ \dots \\ \dots \\ \frac{L^2\,l\,m\,q3\,(m+M)\,\sin(-q2+2\,q1)+l\,L^2\,m\,(q3+q4)}{\dots} \end{array} \right]$$